fr.inria.atlanmod.coqtl.coq/examples/Class2Relational/theorems/thm_table_id_test.v
@@ -1,0 +1,63 @@
+Require Import Coq.Logic.Eqdep_dec.
+Require Import Coq.Arith.EqNat.
+Require Import List.
+From mathcomp Require Import ssreflect ssrfun ssrbool eqtype.
+
+Require Import core.utils.tTop.
+Require Import core.utils.CpdtTactics.
+Require Import core.Notations.
+Require Import core.CoqTL.
+Require Import core.Metamodel.
+Require Import core.Model.
+Require Import core.Model.
+
+Require Import examples.Class2Relational.Class2Relational.
+Require Import examples.Class2Relational.ClassMetamodel.
+Require Import examples.Class2Relational.RelationalMetamodel.
+
+
+
+Theorem Table_id_positive_by_surj :
+  forall (cm : ClassModel) (rm : RelationalModel), 
+    rm = execute Class2Relational cm (* transformation *) ->
+      (forall (c1 : ClassMetamodel_EObject), In c1 (@allModelElements _ _ cm) -> ClassMetamodel_getId c1 > 0) (* precondition *) ->
+        (forall (t1 : RelationalMetamodel_EObject), In t1 (@allModelElements _ _ rm) -> RelationalMetamodel_getId t1 > 0). (* postcondition *)
+Proof.
+  intros cm rm H Hpre t1 Hintm.  
+  remember H as tr.
+  clear Heqtr.
+  apply tr_execute_surj_elements with (t1:=t1) in H.
+  Focus 2. assumption.
+  Focus 1.
+  destruct H as [sp]. destruct H as [tp]. destruct H as [inst].
+  destruct H as [Hinsm]. destruct H as [Hintp]. rename H into Hincltp.
+  apply tr_instantiatePattern_surj_elements with (t1:=t1) (tm:=rm) in inst.
+  - { 
+      destruct inst as [r]. destruct H as [Hrintr]. destruct H as [Hmatch]. rename H into Hinst.
+      destruct sp eqn:sp_ca.
+      -- inversion Hmatch.
+      -- destruct l eqn:l_ca.
+         --- apply tr_instantiateRuleOnPattern_surj_elements with (t1:=t1) (tm:=rm) in Hinst.  
+              ----  destruct Hinst as [Hgpre].
+                    destruct H as [Hguard].
+                    destruct H as [outexpr].
+                    destruct H as [HoutinOuts].
+                    rename H into Heval.
+                    unfold evalOutputPatternElementExpression in Heval.
+
+(* The problem here is that:
+     the signature of evalOutputPatternElementExpression does not have Rule as input,
+     instead it computes a rule based on the given outexpression.
+     so there are at least two Rules in the context, but Coq have no idea they are the same.
+ *)
+                    simpl in Heval.
+                    admit.
+              ---- assumption.
+              ---- assumption.
+              ---- assumption.
+         --- inversion Hmatch.
+    }
+  - assumption.
+  - assumption.
+  - assumption.
+Admitted.
